Eff.Examples.Equations.State.fst
@@ -1,0 +1,92 @@
+module Eff.Examples.Equations.State
+
+module S = Eff.Signature
+
+open Eff.Examples.IntState
+
+open FStar.FunctionalExtensionality
+
+open FStar.Tactics // temporary
+
+
+
+
+
+
+assume val st : Type
+
+let t a = st -> a * st
+
+let return #a (x:a) 
+  : t a 
+  = fun s -> x , s
+
+let read #a (k:st -> t a) 
+  : t a 
+  = fun s -> k s s
+
+let write #a (s:st) (k:unit -> t a)
+  : t a
+  = fun _ -> k () s
+
+
+let st_eq1 #a s (z:st -> t a)
+  : Lemma (normalize (write s (fun _ -> read z) == write s (fun _ -> z s))) 
+  = ()
+
+let st_eq2 #a s s' (z:unit -> t a)
+  : Lemma (normalize (write s (fun _ -> write s' z) == write s' z))
+  = ()
+
+let st_eq3 #a (z:unit -> t a)
+  : Lemma (normalize (read (fun s -> write s z) == z ()))
+  = admit ()
+
+let st_eq3' #a (z:unit -> t a)
+  : Lemma (normalize (read (fun s -> write s z) == (fun s -> z () s)))
+  = ()
+
+
+
+
+
+
+
+
+(*
+
+
+assume val st : Type
+
+let t a = st ^-> a * st
+
+let return #a (x:a) 
+  : t a 
+  = on st (fun s -> x , s)
+
+let read #a (k:st -> t a) 
+  : t a 
+  = on st (fun s -> k s s)
+
+let write #a (s:st) (k:unit -> t a)
+  : t a
+  = on st (fun _ -> k () s)
+
+
+let st_eq1 #a s (z:st ^-> t a)
+  : Lemma (normalize (write s (fun _ -> read z) == write s (fun _ -> z s)))
+  = ()
+
+let st_eq2 #a s s' (z:unit ^-> t a)
+  : Lemma (normalize (write s (fun _ -> write s' z) == write s' z))
+  = ()
+
+let st_eq3 #a (z:unit ^-> t a)
+  : Lemma (normalize (read (fun s -> write s z) == z ()))
+  = ();
+    assert (feq (fun s -> z () s) (z ())
+
+
+*)
+
+
