Eff.Template.Equation.Test2.fst
@@ -1,0 +1,74 @@
+module Eff.Template.Equation.Test2
+
+open Eff.Signature
+open Eff.Template
+open Eff.Template.Equation
+open Eff.Template.Equiv
+
+(* Read and write effects for integer state *)
+
+let read = Op "read" #unit #int
+let write = Op "write" #int #unit
+
+let r : sig = singleton read
+let w : sig = singleton write
+let rw : sig = r `union` w
+
+
+(* Some dummy equations *)
+
+unfold
+let eq1 a x (z:unit -> template_repr a rw) 
+  = Node write x z `equiv` z ()
+
+unfold
+let eq2 a x y (z:unit -> template_repr a rw) 
+  = Node write x z `equiv` Node write y z
+
+
+(* Some experiments re proving equations from eq1 and eq2 *)
+
+assume val t : Type
+
+open FStar.Tactics
+
+let f (z:unit -> template_repr t rw) 
+  : Pure unit 
+         (requires (forall a x z . eq1 a x z))
+         (ensures  (fun _ -> Node write 42 z `equiv` Node write 24 z))
+  = ()
+
+let g (z:unit -> template_repr t rw) 
+  : Pure unit 
+         (requires (forall a x z . eq1 a x z))
+         (ensures  (fun _ -> (Node read () (fun _ -> Node write 42 z)) 
+                          `equiv` 
+                          (Node read () (fun _ -> Node write 24 z))))
+  = ()
+
+let h (z:unit -> template_repr t rw) 
+  : Pure unit 
+         (requires (forall a x z . eq1 a x z))
+         (ensures  (fun _ -> Node read () (fun _ -> Node read () (fun _ -> Node write 42 z))
+                          `equiv`
+                          Node read () (fun _ -> Node read () (fun _ -> Node write 24 z))))
+  = ()
+
+let k (z:unit -> template_repr t rw) 
+  : Pure unit 
+         (requires (forall a x z . eq1 a x z))
+         (ensures  (fun _ -> Node write 24 (fun _ -> Node read () (fun _ -> Node read () ((fun _ -> Node write 42 z))))
+                          `equiv`
+                          Node read () (fun _ -> Node read () (fun _ -> Node write 24 z))))
+  = ()
+
+[@ expect_failure]
+let k' (z:unit -> template_repr t rw) 
+  : Pure unit 
+         (requires (forall a x y z . eq2 a x y z)) // eq2 doesn't justify discarding writes altogether!
+         (ensures  (fun _ -> Node write 24 (fun _ -> Node read () (fun _ -> Node read () ((fun _ -> Node write 42 z))))
+                          `equiv`
+                          Node read () (fun _ -> Node read () (fun _ -> Node write 24 z))))
+  = ()
+
+
