Eff.Template.Equiv.fsti
@@ -1,0 +1,33 @@
+module Eff.Template.Equiv
+
+open Eff.Signature
+open Eff.Template
+
+val equiv (#a:Type) (#ops:sig) (t1 t2:template_repr a ops) : prop
+
+val refl (#a:Type) (#ops:sig) (t:template_repr a ops)
+  : Lemma (t `equiv` t)
+          [SMTPat (t `equiv` t)]
+
+val sym (#a:Type) (#ops:sig) (t1 t2:template_repr a ops)
+  : Lemma (requires (t1 `equiv` t2))
+          (ensures  (t2 `equiv` t1))
+          [SMTPat (t2 `equiv` t1)]
+
+val trans (#a:Type) (#ops:sig) (t1 t2 t3:template_repr a ops)
+  : Lemma (requires (t1 `equiv` t2 /\ t2 `equiv` t3))
+          (ensures  (t1 `equiv` t3))
+          [SMTPat (t1 `equiv` t2); 
+           SMTPat (t1 `equiv` t3)]
+
+val leaf_cong (#a:Type) (#ops:sig) (x1 x2:a)
+  : Lemma (requires (x1 == x2))
+          (ensures  (equiv #a #ops (Leaf x1) (Leaf x2)))
+          [SMTPat (equiv #a #ops (Leaf x1) (Leaf x2))]
+
+val op_cong (#a:Type) (#ops:sig) 
+            (op:op{op `mem` ops}) (x:param_of op) 
+            (t1 t2:arity_of op -> template_repr a ops)
+  : Lemma (requires (forall (y:arity_of op) . t1 y `equiv` t2 y))
+          (ensures  (Node op x t1 `equiv` Node op x t2))
+          [SMTPat (Node op x t1 `equiv` Node op x t2)]
